code/ecdsa/Hacl.Impl.EC.ScalarMult.Radix.fst
@@ -13,6 +13,8 @@ open Spec.ECC.Curves
 open Hacl.Impl.EC.Masking
 
 open Hacl.Spec.EC.Definition
+
+open Hacl.Impl.EC.PointAdd
 open Hacl.Impl.EC.PointDouble
 
 
@@ -85,25 +87,156 @@ let montgomery_ladder_2_precomputed #c #a p scalar tempBuffer =
     )
 
 
+[@ CInline]
+inline_for_extraction noextract  
+val montgomery_ladder_step_radix: 
+   #c: curve ->
+  p: point P256 -> tempBuffer: lbuffer uint64 (size 88) -> 
+  precomputedTable: lbuffer uint64 (size 192) ->
+  scalar:  lbuffer uint8 (size 32) -> 
+  i:size_t{v i < 256} -> 
+  Stack unit
+  (requires fun h -> live h p /\live h tempBuffer /\ live h scalar /\
+    LowStar.Monotonic.Buffer.all_disjoint [loc p;loc tempBuffer; loc scalar])
+  (ensures fun h0 _ h1 -> True)
+
+
+
+let montgomery_ladder_step_radix #c p tempBuffer precomputedTable scalar i =  
+  let bits = getScalar_4_byBit #c scalar i in 
+
+  let pointToAdd = create (size 12) (u64 0) in 
+
+  let invK h (k: nat) = True in 
+  Lib.Loops.for 0ul 16ul invK
+  (fun k -> 
+      let mask = eq_mask (to_u64 bits) (to_u64 k) in 
+      (* eq_mask_lemma d (to_u64 k);  *)
+  
+      let lut_cmb_x = sub precomputedTable (k *! 12) (size 4) in 
+      let lut_cmb_y = sub precomputedTable (k *! 12 +! (size 4)) (size 4) in
+      let lut_cmb_z = sub precomputedTable (k *! 12 +! (size 8)) (size 4) in 
+
+      copy_conditional #c (sub pointToAdd (size 0) (size 4)) lut_cmb_x mask;
+      copy_conditional #c (sub pointToAdd (size 4) (size 4)) lut_cmb_y mask;
+      copy_conditional #c (sub pointToAdd (size 8) (size 4)) lut_cmb_z mask
+      
+      
+      ); 
+      
+  
+  point_double p p tempBuffer;
+  point_double p p tempBuffer;
+  point_double p p tempBuffer;
+  point_double p p tempBuffer;
+
+  point_add pointToAdd p p tempBuffer
+
+
+[@ CInline]
+val generatePrecomputedTable: #c: curve -> b: lbuffer uint64 (size 192) -> publicKey: point c ->
+  tempBuffer: lbuffer uint64 (size 88) -> Stack unit  
+  (requires fun h -> True)
+  (ensures fun h0 _ h1 -> True)
+
+let generatePrecomputedTable #c b publicKey tempBuffer = 
+  let point0 = sub b (size 0) (size 12) in 
+  let point1 = sub b (size 12) (size 12) in 
+  let point2 = sub b (size 24) (size 12) in 
+  let point3 = sub b (size 36) (size 12) in 
+  let point4 = sub b (size 48) (size 12) in 
+  let point5 = sub b (size 60) (size 12) in 
+  let point6 = sub b (size 72) (size 12) in 
+  let point7 = sub b (size 84) (size 12) in 
+  let point8 = sub b (size 96) (size 12) in 
+  let point9 = sub b (size 108) (size 12) in 
+  let point10 = sub b (size 120) (size 12) in 
+  let point11 = sub b (size 132) (size 12) in 
+  let point12 = sub b (size 144) (size 12) in 
+  let point13 = sub b (size 156) (size 12) in 
+  let point14 = sub b (size 168) (size 12) in 
+  let point15 = sub b (size 180) (size 12) in 
+
+  Hacl.Impl.EC.LowLevel.uploadZeroPoint #c point0;
+  Hacl.Impl.EC.LowLevel.copy_point #c publicKey point1;
+  point_double #c publicKey point2 tempBuffer;
+  point_add #c point2 point1 point3 tempBuffer;
+  point_double #c point2 point4 tempBuffer;
+  point_add #c point4 point1 point5 tempBuffer;
+  point_double #c point3 point6 tempBuffer;
+  point_add #c point6 point1 point7 tempBuffer;
+  point_double #c point4 point8 tempBuffer;
+  point_add #c point8 point1 point9 tempBuffer;
+  point_double #c point5 point10 tempBuffer;
+  point_add #c point10 point1 point11 tempBuffer;
+  point_double #c point6 point12 tempBuffer;
+  point_add #c point12 point1 point13 tempBuffer;
+  point_double #c point7 point14 tempBuffer;
+  point_add #c point14 point1 point15 tempBuffer
+
+
+
 inline_for_extraction noextract
-val scalar_multiplication_t_0: #c: curve -> #t:buftype -> q: point c -> p: point c -> result: point c -> 
+val montgomery_ladder_2: #buf_type: buftype -> #c: curve -> p: point c -> 
+  scalar: lbuffer_t buf_type uint8 (size 32) -> 
+  tempBuffer:  lbuffer uint64 (size 88)  -> 
+  precomputedTable: lbuffer uint64 (size 192) ->
+  Stack unit
+  (requires fun h -> True )
+  (ensures fun h0 _ h1 -> modifies (loc p |+| loc tempBuffer) h0 h1)
+
+let montgomery_ladder_2 #a #c p scalar tempBuffer precomputedTable =  
+ let h0 = ST.get() in 
+   push_frame();
+
+     [@inline_let]
+     let spec_ml h0 = _ml_step #c (as_seq h0 scalar) in 
+
+
+     [@inline_let]
+     let inv h (i: nat {i <= 64}) = True in 
+
+
+  let bits =  getScalar_4_byBit #c  scalar (u64 0) in 
+  let pointToStart = sub precomputedTable  (bits *. size 12) (size 12) in 
+
+  copy (sub p (size 0) (size 12)) pointToStart;
+  
+     for 1ul 64ul inv 
+       (fun i -> let h2 = ST.get() in
+   montgomery_ladder_step_radix #c p tempBuffer precomputedTable scalar i
+       );
+   pop_frame()
+
+
+
+
+
+inline_for_extraction noextract
+val scalar_multiplication_t_0: #c: curve -> #t:buftype ->  p: point c -> result: point c -> 
   scalar: scalar_t #t #c -> 
   tempBuffer: lbuffer uint64 (size 17 *! getCoordinateLenU64 c) ->
   Stack unit 
-  (requires fun h -> live h q /\ live h p /\ live h result /\ live h scalar /\ live h tempBuffer /\
+  (requires fun h -> True (* live h q /\ live h p /\ live h result /\ live h scalar /\ live h tempBuffer /\
     LowStar.Monotonic.Buffer.all_disjoint [loc p; loc q; loc tempBuffer; loc scalar] /\
     disjoint q result /\ eq_or_disjoint p result /\ disjoint result tempBuffer /\ disjoint result scalar /\
-    point_eval c h p /\ ~ (isPointAtInfinity (point_as_nat c h p)))
-  (ensures fun h0 _ h1 -> modifies (loc q |+| loc result |+| loc tempBuffer) h0 h1 /\ point_eval c h1 q /\ (
+    point_eval c h p /\ ~ (isPointAtInfinity (point_as_nat c h p)) *))
+  (ensures fun h0 _ h1 -> True (* modifies (loc q |+| loc result |+| loc tempBuffer) h0 h1 /\ point_eval c h1 q /\ (
     let i1 = point_as_nat c h0 p in point_mult_0 i1 0; 
     let pD = fromDomainPoint #c #DH (point_as_nat c h1 q) in
     let r0, r1 = montgomery_ladder_spec_left (as_seq h0 scalar) (pointAtInfinity, i1) in 
-    pD == r0))
+    pD == r0 *))
 
 
-let scalar_multiplication_t_0 #c q p result scalar tempBuffer = ()
-  (* uploadStartPoints q p result;  *)
-  (* montgomery_ladder q result scalar tempBuffer *)
+let scalar_multiplication_t_0 #c p result scalar tempBuffer = 
+(*     let len = getCoordinateLenU64 c in 
+  let q = sub tempBuffer (size 0) (size 3 *! len) in 
+  uploadStartPoints q p result; 
+  montgomery_ladder q result scalar tempBuffer;
+  copy q result *)
+  let bufferPrecomputed = create (size 192) (u64 0) in 
+  generatePrecomputedTable bufferPrecomputed result tempBuffer;
+  montgomery_ladder_2 result scalar tempBuffer bufferPrecomputed
 
 
 inline_for_extraction noextract
