code/ecdsa/Hacl.Impl.EC.LowLevel.fsti
@@ -215,3 +215,9 @@ val mul_atomic: x: uint64 -> y: uint64 -> result: lbuffer uint64 (size 1)
     uint_v result + uint_v h0 * pow2 64 = uint_v x * uint_v y))
 
 
+
+inline_for_extraction noextract
+val copy_point: #c: curve -> p: point c -> result: point c -> Stack unit 
+  (requires fun h -> live h p /\ live h result /\ disjoint p result /\ point_eval c h p) 
+  (ensures fun h0 _ h1 -> modifies (loc result) h0 h1 /\ point_eval c h1 result /\ 
+    point_as_nat c h0 p == point_as_nat c h1 result)
